potential definition of env_rs

compiler/proofs/compilerProofScript.sml
@@ -1,7 +1,7 @@
 open HolKernel bossLib boolLib boolSimps listTheory pairTheory rich_listTheory pred_setTheory arithmeticTheory finite_mapTheory relationTheory sortingTheory stringTheory
 open miscLib miscTheory bigStepTheory semanticPrimitivesTheory bigClockTheory replTheory terminationTheory
 open bytecodeTheory bytecodeExtraTheory bytecodeEvalTheory bytecodeClockTheory bytecodeLabelsTheory bytecodeTerminationTheory
-open intLangTheory toIntLangTheory toBytecodeTheory compilerTheory intLangExtraTheory modLangProofTheory conLangProofTheory intLangProofTheory bytecodeProofTheory compilerTerminationTheory
+open conLangTheory intLangTheory toIntLangTheory toBytecodeTheory compilerTheory intLangExtraTheory modLangProofTheory conLangProofTheory exhLangProofTheory intLangProofTheory bytecodeProofTheory compilerTerminationTheory
 open patLangProofTheory
 val _ = new_theory"compilerProof"
 
@@ -1041,22 +1041,33 @@ val good_labels_def = Define`
     ALL_DISTINCT (FILTER is_Label code) ∧
     EVERY (combin$C $< nl o dest_Label) (FILTER is_Label code)`
 
-(*
 val env_rs_def = Define`
   env_rs ((envM,envC,envE):all_env) ((cnt,s):v count_store) (rs:compiler_state) rd bs ⇔
-    ∃s1 tids exh gtagenv genv genv2.
+    ∃genv s1 tids exh gtagenv s2 genv2.
       to_i1_invariant
-        (FST rs.globals_env) (SND rs.globals_env)
+        genv (FST rs.globals_env) (SND rs.globals_env)
         envM envE (cnt,s) (cnt,s1) (set (MAP FST envM)) ∧
       to_i2_invariant
-        tids envC exh rs.contags_env gtagenv (cnt,s1) (cnt,s2) genv genv2 ∧
-
-    let Cs0 = MAP v_to_Cv (MAP v_to_pat (MAP ARB s2)) in
-    let Cg0 = ARB in
+        tids envC exh (FST rs.contags_env, FST(SND rs.contags_env), ARB:unit, ARB:unit)
+        gtagenv (cnt,s1) (cnt,s2) genv genv2 ∧
+    let Cs0 = MAP (v_to_Cv o v_to_pat o (v_to_exh exh)) s2 in
+    let Cg0 = MAP (OPTION_MAP (v_to_Cv o v_to_pat o (v_to_exh exh))) genv2 in
     ∃Cs Cg.
     LIST_REL syneq Cs0 Cs ∧ LIST_REL (OPTREL syneq) Cg0 Cg ∧
     bs.stack = [] ∧
     Cenv_bs rd ((cnt,Cs),Cg) [] [] 0 bs`
-*)
+
+val env_rs_empty = store_thm("env_rs_empty",
+  ``bs.stack = [] ∧ bs.globals = [] ∧ (∀n. bs.clock = SOME n ⇒ n = ck) ∧ rd.sm = [] ∧ rd.cls = FEMPTY ∧ cs = init_compiler_state ⇒
+    env_rs ([],init_envC,[]) (ck,[]) cs rd bs``,
+  simp[env_rs_def,to_i1_invariant_def,to_i2_invariant_def] >> rw[] >>
+  rw[init_compiler_state_def,get_tagenv_def,cenv_inv_def] >>
+  rw[Once v_to_i1_cases] >> rw[Once v_to_i1_cases] >>
+  rw[Once s_to_i1_cases] >> rw[Once s_to_i1'_cases] >> rw[Once v_to_i1_cases] >>
+  qexists_tac`[]` >>
+  rw[Once genv_to_i2_cases] >>
+  rw[Once s_to_i2_cases] >> rw[Once s_to_i2'_cases] >> rw[Once v_to_i2_cases] >>
+  rw[Cenv_bs_def,env_renv_def,s_refs_def,good_rd_def,FEVERY_ALL_FLOOKUP] >>
+  cheat)
 
 val _ = export_theory()
